safety.thy
@@ -13,15 +13,37 @@ lemma get_effectors_split:
 lemma wf_valid_event_sequence:
   assumes wf: "wellFormed_impl E"
   and eInfo_def: "(events E .[ev]) = Some eInfo"
-shows "valid_event_sequence (event_executionOrder eInfo) (event_snapshot eInfo) (happensBefore E)"
+shows "valid_event_sequence (event_executionOrder eInfo) (event_snapshot eInfo) (happensBeforeE E)"
   by (smt compose_forward_def eInfo_def fmpredD local.wf wellFormed_def wellFormed_impl_def wf_correct_execution_lists_def)
+
+lemma execution_order_in_snapshot:
+  assumes wf: "wellFormed_impl E"
+    and eInfo_def: "(events E .[e]) = Some eInfo"
+    and i: "i < length (event_executionOrder eInfo)"
+shows "fst (event_executionOrder eInfo ! i) \<in> snapshot_events (event_snapshot eInfo)"
+proof -
+
+  have i_in: "event_executionOrder eInfo ! i \<in> set (event_executionOrder eInfo)"
+    by (simp add: i)
+
+  have ves: "valid_event_sequence (event_executionOrder eInfo) (event_snapshot eInfo) (happensBeforeE E)"
+    using eInfo_def local.wf wf_valid_event_sequence by auto
+  hence "0 < snapshot_num (event_snapshot eInfo) (fst (event_executionOrder eInfo ! i))"
+    using i_in by (auto simp add: valid_event_sequence_def)
+
+  thus "fst (event_executionOrder eInfo ! i) \<in> snapshot_events (event_snapshot eInfo)"
+    using fmdom'_notD by fastforce
+
+
+qed
+
 
 lemma show_all_states:
   assumes wf: "wellFormed_impl E"
     and p: "\<And>state effectors exec_order snapshot. \<lbrakk>
           state = executeEffectors effectors initialState effector_impl;
           effectors = get_effectors E exec_order;
-          valid_event_sequence exec_order snapshot (happensBefore E)
+          valid_event_sequence exec_order snapshot (happensBeforeE E)
         \<rbrakk> \<Longrightarrow> P state"
   shows "forallStates E P"
 proof (auto simp add: forallStates_def forallEvents_def compose_forward_def fmpred_iff)
@@ -34,7 +56,7 @@ proof (auto simp add: forallStates_def forallEvents_def compose_forward_def fmpr
   proof (rule p[OF 1])
     show "get_effectors E (event_executionOrder eInfo) = get_effectors E (event_executionOrder eInfo)"
       by simp
-    show "valid_event_sequence (event_executionOrder eInfo) (event_snapshot eInfo) (happensBefore E)"
+    show "valid_event_sequence (event_executionOrder eInfo) (event_snapshot eInfo) (happensBeforeE E)"
       using eInfo_def local.wf wf_valid_event_sequence by auto
 
   qed
@@ -48,19 +70,83 @@ proof (auto simp add: forallStates_def forallEvents_def compose_forward_def fmpr
     have event_effectors_def: "get_effectors E (map (Pair e) [0..<length (event_effectors eInfo)]) = event_effectors eInfo"
       by (auto simp add: get_effectors_def compose_forward_def eInfo_def nth_equalityI)
 
+    have sorted_before: "sorted_partial' (event_executionOrder eInfo) (happensBeforeE E)"
+      using eInfo_def local.wf valid_event_sequence_def wf_valid_event_sequence by blast
+
+
     show "event_state_post eInfo = executeEffectors (get_effectors E (event_executionOrder eInfo@map (\<lambda>i. (e,i)) [0..<length (event_effectors eInfo)] )) initialState effector_impl"
       by (simp add: "1" executeEffectors_split get_effectors_split local.event_effectors_def post_def)
 
     show "get_effectors E (event_executionOrder eInfo @ map (Pair e) [0..<length (event_effectors eInfo)]) = get_effectors E (event_executionOrder eInfo @ map (Pair e) [0..<length (event_effectors eInfo)])"
       by simp
 
-    show "valid_event_sequence (event_executionOrder eInfo @ map (Pair e) [0..<length (event_effectors eInfo)]) (snapshot_update (event_snapshot eInfo) e (length (event_effectors eInfo)) ) (happensBefore E)"
-      apply (auto simp add: valid_event_sequence_def snapshot_update_def fmap_entries_def)
+    have valid_seq: "valid_event_sequence (event_executionOrder eInfo) (event_snapshot eInfo) (happensBeforeE E)"
+      using eInfo_def local.wf wf_valid_event_sequence by blast
 
 
+    have e_notin_snapshot: "e \<notin> snapshot_events (event_snapshot eInfo)"
+      using wf apply (auto simp add: wellFormed_impl_def wellFormed_def wf_acyclic_def fmap_entries_def)
+      by (metis eInfo_def fmlookup_dom'_iff option.distinct(1) option.sel)
 
+    hence e_notin_exec_order: "(e,i) \<notin> set (event_executionOrder eInfo)" for i
+      using valid_event_sequence_def valid_seq by fastforce
+
+    show "valid_event_sequence (event_executionOrder eInfo @ map (Pair e) [0..<length (event_effectors eInfo)]) (snapshot_update (event_snapshot eInfo) e (length (event_effectors eInfo)) ) (happensBeforeE E)"
+      unfolding valid_event_sequence_def proof (intro conjI)
+
+      show " \<forall>(ea, i)\<in>snapshot_entries (snapshot_update (event_snapshot eInfo) e (length (event_effectors eInfo))).
+                \<forall>i'<i. (ea, i') \<in> set (event_executionOrder eInfo @ map (Pair e) [0..<length (event_effectors eInfo)])"
+        using valid_seq by (auto simp add: valid_event_sequence_def snapshot_update_def fmap_entries_def)
+
+      show "\<forall>(e', i)\<in>set (event_executionOrder eInfo @ map (Pair e) [0..<length (event_effectors eInfo)]).
+         i < snapshot_num (snapshot_update (event_snapshot eInfo) e (length (event_effectors eInfo))) e'"
+        using valid_seq e_notin_exec_order by (auto simp add: valid_event_sequence_def snapshot_update_def fmap_entries_def)
+
+      show "sorted_partial' (event_executionOrder eInfo @ map (Pair e) [0..<length (event_effectors eInfo)]) (happensBeforeE E)"
+        apply (auto simp add: sorted_partial'_def nth_append happensBeforeE_def)
+        using  sorted_before apply (simp add: happensBeforeE_def sorted_partial'_def) 
+         apply (auto simp add: happensBeforeP2_def split: if_splits option.splits)
+         apply (metis e_notin_exec_order eq_fst_iff nth_mem)
+        apply (auto simp add: includedIn_def)
+      proof -
+        fix j i x2
+        assume a0: "\<not> j < length (event_executionOrder eInfo)"
+          and a1: "j < length (event_executionOrder eInfo) + length (event_effectors eInfo)"
+          and a2: "i < length (event_executionOrder eInfo)"
+          and a3: "e \<noteq> fst (event_executionOrder eInfo ! i)"
+          and a4: "(events E .[fst (event_executionOrder eInfo ! i)]) = Some x2"
+          and a5: "j - length (event_executionOrder eInfo) < snapshot_num (event_snapshot x2) e"
+        have "event_snapshot x2 \<le> event_snapshot eInfo"
+          using wf apply (auto simp add: wellFormed_impl_def wellFormed_def wf_causallyConsistent_def)
+          apply (drule_tac x="(e, eInfo)" in bspec)
+          apply (simp add: eInfo_def in_fmap_entries)
+          apply (auto split: option.splits)
+          apply (drule_tac x="fst (event_executionOrder eInfo ! i)" in bspec)
+          using wf apply (auto simp add: wellFormed_impl_def wellFormed_def wf_correct_execution_lists_def compose_forward_def)[1]
+           apply (drule_tac x=e and y=eInfo in fmpredD)
+          using eInfo_def apply simp
+           apply (auto simp add:  valid_event_sequence_def)[1]
+           apply (drule_tac x="event_executionOrder eInfo ! i" in bspec) back
+          using a2 apply simp
+
+
+          using  apply blast
+
+          find_theorems fmpred
+
+          apply (simp add: a4 in_fmap_entries)
+          apply (auto split: option.splits)
+
+           apply (simp add: fmap_entries_def)
+
+          sorry (* using causal consistency *)
+        hence "snapshot_num (event_snapshot x2) e = 0"
+          sorry
+        thus "False"
+          using a5 by linarith
+      qed
+    qed
   qed
-
 qed
 
 
